lean/Luffs.lean
@@ -2,6 +2,8 @@ import Luffs.Memory.Layout
 import Luffs.Memory.Iris
 import Luffs.Memory.ConcreteIris
 import Luffs.Memory.Semantics
+import Luffs.Memory.TypedIris
+import Luffs.Memory.Value
 import Luffs.Allocator.TLSF
 import Luffs.Allocator.TLSF.Bitmap
 import Luffs.Allocator.TLSF.FreeList
@@ -9,6 +11,7 @@ import Luffs.Allocator.TLSF.Bins
 import Luffs.Allocator.TLSF.Alloc
 import Luffs.Allocator.TLSF.Ownership
 import Luffs.Allocator.TLSF.Dealloc
+import Luffs.Containers.Box
 
 namespace Luffs
 
